IMLTT/typed/checked/IntroCtx.lean
@@ -1,0 +1,35 @@
+import IMLTT.typed.checked.Elaboration
+
+@[simp]
+def shift : (n : Nat) -> Weak n 0
+  | 0 => Weak.id
+  | n + 1 => Weak.shift <| shift n
+
+example : Tm n :=
+  let t : Tm 0 := Tm.tt
+  (t⌊shift n⌋)
+
+theorem weaken_from_n : (↑₁n↬n) = ↑ₚidₚ := by
+  unfold weaken_from
+  split <;> simp
+
+theorem intro_ctx_type (Γ : Ctx n) :
+    (ε ⊢ T type) → (Γ ctx) → (Γ ⊢  T⌊shift n⌋ type) := by
+  intro hεTtype hΓctx
+  induction Γ with
+  | empty => simpa
+  | @extend n' Γ' A ih =>
+    have hsuccn : shift (n' + 1) = (↑ₚshift n') := rfl
+    rw [hsuccn, ←weakening_shift_id]
+    exact weakening_type (ih (ctx_decr hΓctx)) (ctx_extr hΓctx)
+
+theorem intro_ctx {Γ : Ctx n} :
+    (ε ⊢ t ∶ T) → (Γ ctx) → (Γ ⊢ (t⌊shift n⌋) ∶ T⌊shift n⌋) := by
+  intro htT hΓctx
+  induction Γ with
+  | empty => simpa
+  | @extend n' Γ' A ih =>
+    have : shift (n' + 1) = (↑ₚshift n') := rfl
+    rw [this, ←weakening_shift_id]
+    rw (occs := [2]) [←weakening_shift_id]
+    exact weakening_term (ih (ctx_decr hΓctx)) (ctx_extr hΓctx)
